src/QueueInterface.v
@@ -3,6 +3,7 @@ From Coq Require Import List Lia.
 From Clairvoyance Require Import Core Approx ApproxM List Misc BankersQueue Cost Interfaces Tick.
 
 Import ListNotations.
+Import Tick.Notations.
 
 Set Primitive Projections.
 Set Implicit Arguments.
@@ -32,6 +33,7 @@ Inductive op : Type :=
 Notation Eval := (Eval op value).
 Notation Budget := (Budget op value).
 Notation Exec := (Exec op valueA).
+Notation Demand := (Demand op value valueA).
 Notation ApproxAlgebra := (ApproxAlgebra value valueA).
 Notation Potential := (Potential valueA).
 
@@ -108,6 +110,99 @@ Definition onThunk {a b} (y : b) (f : a -> b) (u : T a) : b :=
   | Thunk x => f x
   end.
 
+Definition forcingD {a b} (y : b) (u : T a) (f : a -> Tick b) : Tick b :=
+  match u with
+  | Undefined => Tick.ret y
+  | Thunk x => f x
+  end.
+
+Definition forceD {a} (y : a) (u : T a) : a :=
+  match u with
+  | Undefined => y
+  | Thunk x => x
+  end.
+
+Lemma less_defined_forceD {a} `{LessDefined a} (x : T a) (y : a) (z : a)
+  : y `less_defined` z ->
+    x `less_defined` Thunk z ->
+    forceD y x `less_defined` z.
+Proof.
+  intros Hy Hx; inv Hx; cbn; auto.
+Qed.
+
+Definition demand : Demand :=
+  fun (o : op) (args : list value) (d : list valueA) => match o, args, d with
+  | Empty, _, _ => Tick.ret (bottom_of (exact args))
+  | Push x, (q :: tl), (outD :: _) =>
+    let outD := forceD (bottom_of (exact (push q x))) outD in
+    let+ (qD, _) := pushD q x outD in
+    Tick.ret (qD :: bottom_of (exact tl))
+  | Pop, (q :: tl), outD =>
+    let outD' := match outD with [] => None | qD' :: _ => Some (Undefined, qD') end in
+    let+ qD := popD q outD' in
+    Tick.ret (qD :: bottom_of (exact tl))
+  | _, _, _ => Tick.ret (bottom_of (exact args))
+  end%tick.
+#[export] Existing Instance demand.
+
+Lemma pd : PureDemand.
+Proof.
+  do 2 red. intros [] [|q qs] [|yD ysD] Hq; try apply bottom_is_least; cbn in Hq |- *.
+  - inv Hq.
+    destruct (Tick.val (pushD q x _)) eqn:EpushD.
+    constructor; [ | apply bottom_is_least ].
+    apply (f_equal fst) in EpushD. cbn in EpushD. rewrite <- EpushD.
+    apply pushD_approx.
+    apply less_defined_forceD; [ apply bottom_is_least | auto ].
+  - constructor; [ | apply bottom_is_least ].
+    unfold valueA. rewrite pop_popD; [ reflexivity | ].
+    destruct pop as [ [] |]; [ inv Hq | reflexivity ].
+  - constructor; [ | apply bottom_is_least ].
+    apply popD_approx. destruct pop as [ [] |]; inv Hq.
+    repeat constructor; auto.
+Qed.
+
+Lemma cd : CvDemand.
+Proof.
+  do 2 red. intros []; cbn.
+  - intros qs yD Hy n xD; injection 1; intros -> ->. unfold emptyA.
+    mgo'. split; [ | auto ]. constructor; assumption.
+  - intros [| q qs] yD Hy; inv Hy.
+    { intros ? ?; injection 1; intros -> ->; cbn; mgo'. split; reflexivity. }
+    intros n xD. destruct pushD as [ ? [] ] eqn:EpushD. intros Hpush; inv Hpush.
+    apply optimistic_bind.
+    assert (t0 = Thunk x); [ | subst t0 ].
+    { apply (f_equal (fun m => snd (Tick.val m))) in EpushD.
+      unfold pushD in EpushD. cbn in EpushD.
+      match goal with [ H : context [ match ?u with _ => _ end ] |- _ ] => destruct u end.
+      cbn in EpushD. auto. }
+    eapply optimistic_mon; [ eapply pushD_spec |].
+    { eapply less_defined_forceD; [ apply bottom_is_least | eassumption ]. }
+    { rewrite EpushD. reflexivity. }
+    cbn beta. intros ? ? []. mforward idtac.
+    split.
+    { constructor; auto. inv H2; cbn in H; constructor; auto. }
+    { rewrite EpushD in H0. cbn in H0. lia. }
+  - intros [| q qs] yD Hy.
+    { intros ? ? Hd; inv Hd; cbn. mforward idtac. split; auto. }
+    destruct popD eqn:EpopD. intros ? ? Hd; inv Hd.
+    mforward idtac.
+    match goal with [ HH : _ _ ?w = _ |- _ ] => pose (v := w); fold v in HH end.
+    eapply optimistic_mon; [ eapply popD_spec | ].
+    2:{ apply (eq_sym (f_equal Tick.val EpopD)). }
+    { destruct pop as [ [] | ].
+      { inv Hy. repeat constructor; auto. }
+      { inv Hy. reflexivity. } }
+    cbn beta. intros ? ? [Hdef Hcost].
+    rewrite EpopD in Hcost; simpl in Hcost.
+    destruct (pop q) as [ [] | ] eqn:Hpop; inv Hy; inv Hdef.
+    + destruct y. mforward idtac. split; [ | lia ].
+      { constructor; [ apply H0 | auto ]. }
+    + mforward idtac. split; [ reflexivity | lia ].
+Qed.
+
+#[export] Existing Instances pd cd.
+
 (* "debt" in BankersQueue *)
 Definition potential : Potential := (* ... *)
   onThunk 0 (fun qA => 2 * sizeX 0 (frontA qA) - 2 * nbackA qA).
@@ -150,78 +245,40 @@ Proof.
   cbn in Ev. inv Ev. auto.
 Qed.
 
-Theorem physicist's_argument : Physicist'sArgument.
+Theorem physicist's_argumentD : Physicist'sArgumentD.
 Proof.
-  red. intros [] vs Hvs output Houtput; cbn [exec].
-  - exists (bottom_of (exact vs)).
-    split; [ apply bottom_is_least | ].
-    unfold emptyA; mgo_.
-    split; [ assumption | ].
-    replace (sumof _ _) with 0.
-    2: symmetry; apply (potential_bottom_list (approx_algebra := approx_algebra) potential_bottom _).
-    lia.
-  - destruct vs; cbn [eval] in Houtput.
-    { exists []; split; [ constructor | ].
-      mgo_. split; auto. lia. }
-    inv Houtput. inv H3.
-    exists (fst (Tick.val (pushD v x (onThunk (bottom_of (exact (push v x))) (fun q => q) x0))) :: bottom_of (exact vs)).
-    split.
-    { constructor.
-      { apply pushD_approx. inv H2; cbn. { apply bottom_is_least. } { assumption. } }
-      { apply bottom_is_least. } }
-    mgo_.
-    inv Hvs.
-    relax.
-    { eapply pushA_cost'.
-      - eassumption.
-      - apply less_defined_onThunk in H2. exact H2.
-      - apply pushD_val.
-      - reflexivity. }
-    cbn beta; intros ? ? [HH1 HH2]. change (debt (a := T _)) with potential in HH2.
-    replace (debt (onThunk _ _ _)) with (potential x0) in HH2.
-    2:{ destruct x0; reflexivity. }
-    mgo_.
-    split.
-    { constructor; [ | constructor ]. revert HH1. apply less_defined_onThunk_inv. }
-    remember (potential _).
-    replace (sumof _ _) with 0; [ lia | ].
-    symmetry; apply (sumof_bottom (Hf_bottom := @potential_bottom _ _ _ _ well_defined_potential)).
-  - destruct vs; cbn [eval] in Houtput.
-    { exists []; split; [ constructor | ].
-      mgo_. split; auto. lia. }
-    pose (outD := match output with [] => None | q :: _ => Some (@Undefined a, q) end).
-    pose (inD := Tick.val (popD v outD)).
-    exists (inD :: bottom_of (exact vs)).
-    split.
-    { constructor.
-      + apply popD_approx.
-        destruct pop as [ [] | ]; inv Houtput.
-        { constructor; constructor; constructor + assumption. }
-        { constructor. }
-      + apply bottom_is_least. }
-    mgo_.
-    inv Hvs.
-    relax.
-    { eapply (popA_cost' (outD := outD)).
-      - eassumption.
-      - destruct pop as [ [] | ]; inv Houtput.
-        + constructor. constructor; [ constructor | ]. auto.
-        + constructor.
-      - reflexivity. }
-    cbn beta.
-    intros ? ? [HH1 HH2].
-    change (debt (Tick.val (popD v outD))) with (potential inD) in HH2.
-    destruct pop as [ [] | ]; inv Houtput.
-    + inv HH1. inv H5. destruct y. mgo_.
-      split; [ constructor; [apply H0 | constructor ] | ].
-      change (debt x0) with (potential x0) in HH2.
-      replace (sumof _ _) with 0; [ lia | ].
-      symmetry; apply (sumof_bottom (Hf_bottom := @potential_bottom _ _ _ _ well_defined_potential)).
-    + inv HH1. mgo_. split; [ constructor | ].
-      replace (sumof _ _) with 0; [ lia | ].
-      symmetry; apply (sumof_bottom (Hf_bottom := @potential_bottom _ _ _ _ well_defined_potential)).
+  assert (Hsp : forall v, sumof potential (bottom_of v) = 0).
+  { apply (sumof_bottom (Hf_bottom := @potential_bottom _ _ _ _ well_defined_potential)). }
+  red. intros [] vs Hvs output Houtput; cbn [demand].
+  - intros ? ? Hd; inv Hd. rewrite Hsp. lia.
+  - destruct vs; intros ? ? Hd.
+    { inv Hd. rewrite Hsp; lia. }
+    destruct output.
+    { inv Hd. rewrite Hsp; lia. }
+    destruct pushD as [ ? [] ] eqn:EpushD in Hd. inv Hd.
+    cbn. rewrite Hsp. inv Hvs.
+    inv Houtput. inv H6.
+    unshelve eassert (HH := pushD_cost H1 _ (f_equal Tick.val (eq_sym EpushD))).
+    { apply less_defined_forceD; [ apply bottom_is_least | auto ]. }
+    rewrite EpushD in HH. cbn [Tick.cost] in HH. cbn [sumof fold_right].
+    change (potential t) with (debt t).
+    destruct v0; cbn [forceD] in HH.
+    { change (potential (Thunk x0)) with (debt x0). lia. }
+    { cbn. change (debt (bottom_of ?w)) with 0 in HH. lia. }
+  - destruct vs; intros ? ? Hd.
+    { inv Hd; rewrite Hsp; lia. }
+    destruct popD as [] eqn:EpopD in Hd. inv Hd. cbn.
+    rewrite Hsp. inv Hvs.
+    cbn in Houtput.
+    lazymatch goal with [ HH : _ _ ?ww = _ |- _ ] => pose (w := ww); fold w in EpopD end.
+    unshelve eassert (HH := popD_cost (outD := w) H1 _).
+    { destruct pop as [ [] | ]; inv Houtput; repeat constructor; cbn; auto. }
+    rewrite EpopD in HH; cbn [Tick.val Tick.cost] in HH.
+    match type of HH with (_ <= _ + ?z) => replace z with (sumof potential output) in HH end.
+    { change (potential val) with (debt val). lia. }
+    { destruct pop as [ [] | ]; inv Houtput; [ | auto ]. inv H5. cbn. auto. }
 Qed.
-#[export] Existing Instance physicist's_argument.
+#[export] Existing Instance physicist's_argumentD.
 
 Theorem amortized_cost : AmortizedCostSpec.
 Proof. apply physicist's_method. Qed.
